wip

LeanSubst/Ren.lean
@@ -8,67 +8,94 @@ namespace LeanSubst
 
   def Ren.id : Ren := ⟨λ x => x⟩
 
+  @[simp]
+  theorem Ren.id_action {x} : id.act x = x := by simp [Ren.id]
+
+  def Ren.succ : Ren := ⟨(· + 1)⟩
+
+  @[simp]
+  theorem Ren.succ_action {x} : succ.act x = x + 1 := by simp [Ren.succ]
+
+  def Ren.pred : Ren := ⟨(· - 1)⟩
+
+  @[simp]
+  theorem Ren.pred_action {x} : pred.act x = x - 1 := by simp [Ren.pred]
+
   def Ren.add (k : Nat) : Ren := ⟨(· + k)⟩
+
+  @[simp]
+  theorem Ren.add_action {k x} : (add k).act x = x + k := by simp [Ren.add]
+
+  @[simp]
+  theorem Ren.add_zero : add 0 = id := by simp [Ren.add, Ren.id]
+
+  @[simp]
+  theorem Ren.add_one : add 1 = succ := by simp [Ren.add, Ren.succ]
 
   def Ren.sub (k : Nat) : Ren := ⟨(· - k)⟩
 
-  def Ren.lift (r : Ren) (k : Nat := 1) : Ren := .mk λ n =>
-    if n < k then n else r.act (n - k) + k
+  @[simp]
+  theorem Ren.sub_action {k x} : (sub k).act x = x - k := by simp [Ren.sub]
+
+  @[simp]
+  theorem Ren.sub_zero : sub 0 = id := by simp [Ren.sub, Ren.id]
+
+  @[simp]
+  theorem Ren.sub_one : sub 1 = pred := by simp [Ren.sub, Ren.pred]
 
   def Ren.cons (a : Nat) (r : Ren) : Ren := .mk λ n =>
     match n with
     | 0 => a
     | n + 1 => r.act n
 
+  infixr:67 (name := Ren.cons_notation) " :: " => Ren.cons
+
+  @[simp]
+  theorem Ren.cons_action0 {a} {r : Ren} : (a::r).act 0 = a := by simp [Ren.cons]
+
+  @[simp]
+  theorem Ren.cons_action {a i} {r : Ren} : (a::r).act (i + 1) = r.act i := by simp [Ren.cons]
+
   def Ren.append : List Nat -> Ren -> Ren
   | .nil, r => r
-  | .cons hd tl, r => append tl (r.cons hd)
+  | .cons hd tl, r => hd::append tl r
 
   instance : HAppend (List Nat) Ren Ren where
     hAppend := Ren.append
 
+  @[simp]
+  theorem Ren.append_nil {r : Ren} : ([] : List Nat) ++ r = r := by
+    simp [HAppend.hAppend, Ren.append]
+
+  @[simp]
+  theorem Ren.append_cons {a} {ℓ : List Nat} {r : Ren} : (a::ℓ) ++ r = a::(ℓ ++ r) := by
+    simp [HAppend.hAppend, Ren.append]
+
+  @[simp, grind <-]
+  theorem Ren.append_action_lt {r : Ren} {i}
+    : {ℓ : List Nat} -> (h : i < ℓ.length) -> (ℓ ++ r).act i = ℓ[i]
+  | .cons hd tl, h =>
+    match i with
+    | 0 => rfl
+    | i + 1 => append_action_lt (r := r) (ℓ := tl) (by grind)
+
+  @[simp, grind =]
+  theorem Ren.append_action_ge {r : Ren} {i}
+    : {ℓ : List Nat} -> (h : i ≥ ℓ.length) -> (ℓ ++ r).act i = r.act (i - ℓ.length)
+  | .nil, h => by simp
+  | .cons hd tl, h =>
+    match i with
+    | 0 => by simp at h
+    | i + 1 => @append_action_ge r i tl (by grind) |> cast (by simp)
+
   def Ren.compose : Ren -> Ren -> Ren
   | r1, r2 => .mk λ n => r2.act (r1.act n)
 
-  class RenMap (T : Type) where
-    rmap : Ren -> T -> T
-
-  export RenMap (rmap)
-
-  macro:max t:term noWs "⟨" r:term "⟩" : term => `(rmap $r $t)
-  infixr:67 (name := Ren.cons_notation) " :: " => Ren.cons
   infixr:85 (name := Ren.compose_notation) " ∘ " => Ren.compose
 
-  @[app_unexpander rmap]
-  def unexpandRenApply : Lean.PrettyPrinter.Unexpander
-  | `($_ $r $t) => `($t⟨$r⟩)
-  | _ => throw ()
-
-  @[simp, grind =]
-  theorem Ren.lift_zero {r : Ren} : r.lift 0 = r := by
-    unfold Ren.lift; congr
-
-  @[grind =]
-  theorem Ren.lift_succ {r : Ren} {k} : r.lift (k + 1) = (r.lift k).lift := by
-    induction k; simp
-    case _ n ih =>
-      unfold Ren.lift; congr; funext; case _ i =>
-      simp; unfold Ren.lift at ih; simp at ih
-      grind
-
   @[simp]
-  theorem Ren.id_action {x} : Ren.id.act x = x := by simp [Ren.id]
-
-  @[simp]
-  theorem Ren.lift_id {k} : Ren.lift Ren.id k = Ren.id := by
-    simp [Ren.id, Ren.lift]; congr; funext; case _ x =>
-    cases x <;> simp; omega
-
-  @[simp]
-  theorem Ren.cons_head_action {n} {r : Ren} : (n::r).act 0 = n := by simp [Ren.cons]
-
-  @[simp]
-  theorem Ren.cons_tail_action {n i} {r : Ren} : (n::r).act (i + 1) = r.act i := by simp [Ren.cons]
+  theorem Ren.compose_action {r1 r2 : Ren} {x} : (r1 ∘ r2).act x = r2.act (r1.act x) := by
+    simp [Ren.compose]
 
   @[simp]
   theorem Ren.compose_id_left {r : Ren} : id ∘ r = r := by
@@ -82,9 +109,33 @@ namespace LeanSubst
   theorem Ren.compose_assoc {r1 r2 r3 : Ren} : (r1 ∘ r2) ∘ r3 = r1 ∘ r2 ∘ r3 := by
     simp [Ren.compose]
 
+  def Ren.lift (r : Ren) (k : Nat := 1) : Ren := .mk λ n =>
+    if n < k then n else r.act (n - k) + k
+
+  @[simp, grind <-]
+  theorem Ren.lift_action_lt {r k i} (h : i < k) : (lift r k).act i = i := by
+    simp [Ren.lift]; grind
+
+  @[simp, grind <-]
+  theorem Ren.lift_action_ge {r k i} (h : i ≥ k) : (lift r k).act i = r.act (i - k) + k := by
+    simp [Ren.lift]; grind
+
   @[simp]
-  theorem Ren.compose_action {r1 r2 : Ren} {x} : (r1 ∘ r2).act x = r2.act (r1.act x) := by
-    simp [Ren.compose]
+  theorem Ren.lift_of_zero {r : Ren} : r.lift 0 = r := by
+    unfold Ren.lift; congr
+
+  @[grind =]
+  theorem Ren.lift_of_succ {r : Ren} {k} : r.lift (k + 1) = (r.lift k).lift := by
+    induction k; simp
+    case _ n ih =>
+      unfold Ren.lift; congr; funext; case _ i =>
+      simp; unfold Ren.lift at ih; simp at ih
+      grind
+
+  @[simp]
+  theorem Ren.lift_id {k} : Ren.lift Ren.id k = Ren.id := by
+    simp [Ren.id, Ren.lift]; congr; funext; case _ x =>
+    cases x <;> simp; omega
 
   theorem Ren.compose_lift_k1 {r1 r2 : Ren} : (r1 ∘ r2).lift = r1.lift ∘ r2.lift := by
     simp [Ren.compose, Ren.lift]
@@ -95,10 +146,22 @@ namespace LeanSubst
   theorem Ren.compose_lift {k} {r1 r2 : Ren} : (r1 ∘ r2).lift k = r1.lift k ∘ r2.lift k := by
     induction k generalizing r1 r2; simp
     case _ k ih =>
-      rw [lift_succ, ih]
-      rw [lift_succ (r := r1)]
-      rw [lift_succ (r := r2)]
+      rw [lift_of_succ, ih]
+      rw [lift_of_succ (r := r1)]
+      rw [lift_of_succ (r := r2)]
       rw [compose_lift_k1]
+
+  class RenMap (T : Type) where
+    rmap : Ren -> T -> T
+
+  export RenMap (rmap)
+
+  macro:max t:term noWs "⟨" r:term "⟩" : term => `(rmap $r $t)
+
+  @[app_unexpander rmap]
+  def unexpandRenApply : Lean.PrettyPrinter.Unexpander
+  | `($_ $r $t) => `($t⟨$r⟩)
+  | _ => throw ()
 
   class RenMapId (S : Type) [RenMap S] where
     apply_id {t : S} : t⟨Ren.id⟩ = t
@@ -106,7 +169,7 @@ namespace LeanSubst
   class RenMapCompose (S : Type) [RenMap S] where
     apply_compose {s : S} {r1 r2 : Ren} : s⟨r1⟩⟨r2⟩ = s⟨r1 ∘ r2⟩
 
-  @[simp, grind =]
+  @[simp]
   theorem Ren.apply_id [RenMap T] [RenMapId T] {t : T} : t⟨id⟩ = t := RenMapId.apply_id
 
   @[simp, grind =]
