LeanSubst/Subst.lean
@@ -11,8 +11,172 @@ namespace LeanSubst
 
   export Subst.Action (re su)
 
+  @[simp]
+  def Subst.Action.rmap {T} [RenMap T] (r : Ren) : Subst.Action T -> Subst.Action T
+  | re x => re $ r.act x
+  | su t => su t⟨r⟩
+
+  instance [RenMap T] : RenMap (Subst.Action T) where
+    rmap := Subst.Action.rmap
+
+  @[simp]
+  theorem Subst.Action.rmap_re [RenMap T] {r} {x : Nat}
+    : (@re T x)⟨r⟩ = re (r.act x)
+  := by simp [RenMap.rmap]
+
+  @[simp]
+  theorem Subst.Action.rmap_su [RenMap T] {r} {t : T} : (su t)⟨r⟩ = su t⟨r⟩ := by
+    simp [RenMap.rmap]
+
+  instance [RenMap T] [RenMapId T] : RenMapId (Subst.Action T) where
+    apply_id := by
+      intro t; simp [RenMap.rmap]
+      cases t <;> simp
+
+  instance [RenMap T] [RenMapCompose T] : RenMapCompose (Subst.Action T) where
+    apply_compose := by
+      intro s r1 r2; simp [RenMap.rmap, Ren.compose]
+      cases s <;> simp [Ren.compose]
+
   structure Subst (T : Type) where
     act : Nat -> Subst.Action T
+
+  def Subst.id : Subst T := ⟨λ x => re x⟩
+  notation "+0" => Subst.id
+
+  @[simp]
+  theorem Subst.id_action {x} : (@Subst.id T).act x = re x := by simp [Subst.id]
+
+  def Subst.succ : Subst T := ⟨λ x => re $ x + 1⟩
+  notation "+1" => Subst.succ
+
+  @[simp]
+  theorem Subst.succ_action {x} : (@Subst.succ T).act x = re (x + 1) := by simp [Subst.succ]
+
+  def Subst.pred : Subst T := ⟨λ x => re $ x - 1⟩
+  notation "-1" => Subst.pred
+
+  @[simp]
+  theorem Subst.pred_action {x} : (@Subst.pred T).act x = re (x - 1) := by simp [Subst.pred]
+
+  def Subst.add (k : Nat) : Subst T := ⟨λ x => re $ x + k⟩
+
+  @[simp]
+  theorem Subst.add_action {k x} : (@Subst.add T k).act x = re (x + k) := by simp [Subst.add]
+
+  @[simp]
+  theorem Subst.add_zero : add 0 = @id T := by simp [Subst.add, Subst.id]
+
+  @[simp]
+  theorem Subst.add_one : add 1 = @succ T := by simp [Subst.add, Subst.succ]
+
+  def Subst.sub (k : Nat) : Subst T := ⟨λ x => re $ x - k⟩
+
+  @[simp]
+  theorem Subst.sub_action {k x} : (@Subst.sub T k).act x = re (x - k) := by simp [Subst.sub]
+
+  @[simp]
+  theorem Subst.sub_zero : sub 0 = @id T := by simp [Subst.sub, Subst.id]
+
+  @[simp]
+  theorem Subst.sub_one : sub 1 = @pred T := by simp [Subst.sub, Subst.pred]
+
+  def Subst.cons (a : Subst.Action T) (σ : Subst T) : Subst T := .mk λ n =>
+    match n with
+    | 0 => a
+    | n + 1 => σ.act n
+
+  infixr:67 (name := Subst.cons_notation) " :: " => Subst.cons
+
+  @[simp]
+  theorem Subst.cons_action0 {a} {σ : Subst T} : (a::σ).act 0 = a := by simp [Subst.cons]
+
+  @[simp]
+  theorem Subst.cons_action {a i} {σ : Subst T} : (a::σ).act (i + 1) = σ.act i := by
+    simp [Subst.cons]
+
+  def Subst.append : List (Subst.Action T) -> Subst T -> Subst T
+  | .nil, σ => σ
+  | .cons hd tl, σ => hd::append tl σ
+
+  instance : HAppend (List $ Subst.Action T) (Subst T) (Subst T) where
+    hAppend := Subst.append
+
+  @[simp]
+  theorem Subst.append_nil {σ : Subst T} : ([] : List $ Action T) ++ σ = σ := by
+    simp [HAppend.hAppend, Subst.append]
+
+  @[simp]
+  theorem Subst.append_cons {a} {ℓ : List (Action T)} {σ : Subst T}
+    : (a::ℓ) ++ σ = a::(ℓ ++ σ)
+  := by simp [HAppend.hAppend, Subst.append]
+
+  @[simp, grind <-]
+  theorem Subst.append_action_lt {σ : Subst T} {i}
+    : {ℓ : List $ Action T} -> (h : i < ℓ.length) -> (ℓ ++ σ).act i = ℓ[i]
+  | .cons hd tl, h =>
+    match i with
+    | 0 => rfl
+    | i + 1 => append_action_lt (σ := σ) (ℓ := tl) (by grind)
+
+  @[simp, grind =]
+  theorem Subst.append_action_ge {σ : Subst T} {i}
+    : {ℓ : List $ Action T} -> (h : i ≥ ℓ.length) -> (ℓ ++ σ).act i = σ.act (i - ℓ.length)
+  | .nil, h => by simp
+  | .cons hd tl, h =>
+    match i with
+    | 0 => by simp at h
+    | i + 1 => @append_action_ge σ i tl (by grind) |> cast (by simp)
+
+  class SubstMap (S T : Type) where
+    smap : Subst T -> S -> S
+
+  export SubstMap (smap)
+
+  macro:max t:term noWs "[" σ:term "]" : term => `(smap $σ $t)
+
+  @[app_unexpander smap]
+  def unexpandSubstApply : Lean.PrettyPrinter.Unexpander
+  | `($_ $σ $t) => `($t[$σ])
+  | _ => throw ()
+
+  def Subst.compose [RenMap T] [SubstMap T T] : Subst T -> Subst T -> Subst T
+  | σ, τ => .mk λ n =>
+    match σ.act n with
+    | su t => su t[τ]
+    | re k => τ.act k
+
+  infixr:85 (name := Subst.compose_notation) " ∘ " => Subst.compose
+
+  def Subst.lift [RenMap T] (σ : Subst T) (k : Nat := 1) : Subst T := .mk λ n =>
+    if n < k then re n else (σ.act (n - k))⟨.add k⟩
+
+  @[simp, grind <-]
+  theorem Subst.lift_action_lt [RenMap T] {σ : Subst T} {k i} (h : i < k)
+    : (lift σ k).act i = re i
+  := by simp [Subst.lift]; grind
+
+  @[simp, grind <-]
+  theorem Subst.lift_action_ge [RenMap T] {σ : Subst T} {k i} (h : i ≥ k)
+    : (lift σ k).act i = (σ.act (i - k))⟨.add k⟩
+  := by simp [Subst.lift]; grind
+
+  -- @[simp]
+  -- theorem Subst.lift_of_zero [RenMap T] [RenMapId T] {σ : Subst T} : σ.lift 0 = σ := by
+  --   unfold Subst.lift; congr; simp
+
+  -- @[grind =]
+  -- theorem Subst.lift_of_succ [RenMap T] [RenMapId T] {σ : Subst T} {k} : σ.lift (k + 1) = (σ.lift k).lift := by
+  --   induction k; simp
+  --   case _ n ih =>
+  --     unfold Subst.lift; congr; funext; case _ i =>
+  --     simp; unfold Subst.lift at ih; simp at ih
+  --     grind
+
+  -- @[simp]
+  -- theorem Subst.lift_id {k} : Subst.lift Subst.id k = Subst.id := by
+  --   simp [Subst.id, Subst.lift]; congr; funext; case _ x =>
+  --   cases x <;> simp; omega
 
   @[coe]
   def Ren.to : Ren -> Subst T
@@ -21,82 +185,26 @@ namespace LeanSubst
   instance : Coe Ren (Subst T) where
     coe := Ren.to
 
-  class SubstMap (S T : Type) where
-    smap : Subst T -> S -> S
-
-  export SubstMap (smap)
-
-  def Subst.lift [RenMap T] (σ : Subst T) (k : Nat := 1) : Subst T := .mk λ n =>
-    if n < k then re n else
-      match σ.act (n - k) with
-      | su t => su (rmap (Ren.add k) t)
-      | re i => re (i + k)
-
-  def Subst.cons (a : Subst.Action T) (σ : Subst T) : Subst T := .mk λ n =>
-    match n with
-    | 0 => a
-    | n + 1 => σ.act n
-
-  def Subst.append : List (Subst.Action T) -> Subst T -> Subst T
-  | .nil, σ => σ
-  | .cons hd tl, σ => append tl (σ.cons hd)
-
-  instance : HAppend (List $ Subst.Action T) (Subst T) (Subst T) where
-    hAppend := Subst.append
-
-  @[simp]
-  abbrev smap1 [SubstMap S S] := smap (S := S) (T := S)
-
-  def Subst.compose [RenMap T] [SubstMap T T] : Subst T -> Subst T -> Subst T
-  | σ, τ => .mk λ n =>
-    match σ.act n with
-    | su t => su (smap τ t)
-    | re k => τ.act k
-
-  def Subst.hcompose [RenMap T] [SubstMap S T] : Subst S -> Subst T -> Subst S
-  | σ, τ => .mk λ n =>
-    match σ.act n with
-    | su t => su (smap τ t)
-    | re k => re k
-
-  def Subst.id : Subst T := ⟨λ n => re n⟩
-  def Subst.succ : Subst T := ⟨λ n => re (n + 1)⟩
-  def Subst.pred : Subst T := ⟨λ n => re (n - 1)⟩
-
-  notation "+0" => Subst.id
-  macro "+0@" noWs T:term : term =>`(@Subst.id $T)
-  notation "+1" => Subst.succ
-  macro "+1@" noWs T:term : term =>`(@Subst.succ $T)
-  notation "-1" => Subst.pred
-  macro "-1@" noWs T:term : term =>`(@Subst.pred $T)
+  @[simp, grind =]
+  theorem Ren.to_id : Ren.to (T := T) id = +0 := by simp [Ren.to, Subst.id, id]
 
   @[simp, grind =]
-  theorem Subst.id_action {n} : (+0@T).act n = re n := by simp [Subst.id]
+  theorem Ren.to_succ : Ren.to (T := T) succ = +1 := by simp [Ren.to, Subst.succ]
 
   @[simp, grind =]
-  theorem Subst.succ_action {n} : (+1@T).act n = re (n + 1) := by simp [Subst.succ]
+  theorem Ren.to_pred : Ren.to (T := T) pred = -1 := by simp [Ren.to, Subst.pred]
 
   @[simp, grind =]
-  theorem Subst.pred_action {n} : (-1@T).act n = re (n - 1) := by simp [Subst.pred]
+  theorem Ren.to_add {k} : Ren.to (T := T) (add k) = Subst.add k := by simp [Ren.to, Subst.add]
 
   @[simp, grind =]
-  theorem Ren.to_id : Ren.to (T := T) id = +0 := by
-    unfold Ren.to; unfold Subst.id; simp [id]
-
-  @[simp, grind =]
-  theorem Ren.to_succ : Ren.to (T := T) (Ren.add 1) = +1 := by
-    unfold Ren.to; simp; unfold Subst.succ; simp [Ren.add]
-
-  @[simp, grind =]
-  theorem Ren.to_pred : Ren.to (T := T) (Ren.sub 1) = -1 := by
-    unfold Ren.to; simp; unfold Subst.pred; simp [Ren.sub]
+  theorem Ren.to_sub {k} : Ren.to (T := T) (sub k) = Subst.sub k := by simp [Ren.to, Subst.sub]
 
   @[simp, grind =]
   theorem Ren.pred_succ [RenMap T] [SubstMap T T] : Subst.compose (T := T) +1 -1 = +0 := by
-    unfold Subst.compose; simp
-    unfold Subst.id; rfl
+    simp [Subst.compose, Subst.id]
 
-  @[grind =]
+  @[simp, grind =]
   theorem Ren.to_lift [RenMap T] {r : Ren} {k} : (r.lift k).to = (@Ren.to T r).lift k := by
     cases r; simp [Ren.lift, Ren.to, Subst.lift]; case _ act =>
     funext; case _ x =>
@@ -104,34 +212,23 @@ namespace LeanSubst
     case zero => grind
     case _ n => cases Nat.decLt (n + 1) k <;> simp [ite]
 
-  macro:max t:term noWs "[" σ:term "]" : term => `(smap1 $σ $t)
-  macro:max t:term noWs "[" σ:term ":" T:term "]" : term => `(smap (T := $T) $σ $t)
-  infixr:67 (name := Subst.cons_notation) " :: " => Subst.cons
-  infixr:85 (name := Subst.compose_notation) " ∘ " => Subst.compose
-  infixr:85 " ◾ " => Subst.hcompose
-
-  @[app_unexpander smap1]
-  def unexpandSubstApply1 : Lean.PrettyPrinter.Unexpander
-  | `($_ $σ $t) => `($t[$σ])
-  | _ => throw ()
-
-  @[app_unexpander smap]
-  def unexpandSubstApply : Lean.PrettyPrinter.Unexpander
-  | `($_ $σ $t) => `($t[$σ : _])
-  | `($_ (T := $T) $σ $t) => `($t[$σ : $T])
-  | _ => throw ()
-
   @[simp, grind =]
   theorem Ren.to_compose {r1 r2 : Ren} [RenMap T] [SubstMap T T]
-    : Ren.to (T := T) (r1 ∘ r2) = Subst.compose r1 r2
+    : Ren.to (T := T) (r1 ∘ r2) = r1.to ∘ r2.to
   := by
     funext; case _ x =>
     cases x <;> simp [Ren.to, Subst.compose, Ren.compose]
 
-  @[simp]
-  theorem Subst.cons_head_action {t} {σ : Subst T} : (t::σ).act 0 = t := by simp [Subst.cons]
+  -- def Subst.hcompose [RenMap T] [SubstMap S T] : Subst S -> Subst T -> Subst S
+  -- | σ, τ => .mk λ n =>
+  --   match σ.act n with
+  --   | su t => su (smap τ t)
+  --   | re k => re k
 
-  @[simp]
-  theorem Subst.cons_tail_action {t i} {σ : Subst T} : (t::σ).act (i + 1) = σ.act i := by simp [Subst.cons]
+  -- infixr:85 " ◾ " => Subst.hcompose
+
+  -- macro "+0@" noWs T:term : term =>`(@Subst.id $T)
+  -- macro "+1@" noWs T:term : term =>`(@Subst.succ $T)
+  -- macro "-1@" noWs T:term : term =>`(@Subst.pred $T)
 
 end LeanSubst
