LeanSubst/Types.lean
@@ -1,0 +1,24 @@
+
+namespace LeanSubst
+  universe u1 u2
+  variable {S : Type u1} {T : Type u2}
+
+  structure Ren where
+    act : Nat -> Nat
+
+  structure HetRen (T : Type u1) where
+    act : Nat -> Nat
+
+  inductive Subst.Action (T : Type u1) where
+  | re : Nat -> Subst.Action T
+  | su : T -> Subst.Action T
+  deriving Repr
+
+  export Subst.Action (re su)
+
+  structure Subst (T : Type u1) where
+    act : Nat -> Subst.Action T
+
+
+
+end LeanSubst
